Completing definitions in soundness/ to implement the behavior preservation theorem. Minor changes in hvhdl/ and common/

soundness/SoundnessDefs.v
@@ -3,11 +3,17 @@
 (* Common libraries *)
 
 Require Import common.Coqlib.
+Require Import common.GlobalTypes.
+Require Import common.GlobalFacts.
+Require Import common.ListsPlus.
 
 (* SITPN Libraries *)
 
 Require Import dp.SitpnTypes.
 Require Import dp.Sitpn.
+Require Import dp.SitpnFacts.
+Require Import dp.SitpnSemanticsDefs.
+Require Import dp.Fired.
 
 (* H-VHDL Libraries *)
 
@@ -21,6 +27,10 @@ Require Import hvhdl.SynchronousEvaluation.
 Require Import hvhdl.Initialization.
 Require Import hvhdl.Stabilize.
 
+(* SITPN-to-H-HVDL libraries *)
+
+Require Import sitpn2hvhdl.Sitpn2HVhdlTypes.
+
 (** Defines the relation stating that an SITPN execution environment
     and a H-VHDL design execution environment described the same
     behavior.
@@ -32,30 +42,226 @@ Require Import hvhdl.Stabilize.
     ports of design [d] that implements the conditions of [sitpn].
 *)
 
-Definition EnvEq sitpn (Ec : nat -> C sitpn -> bool) (Ep : nat -> Clk -> IdMap value) : Prop := True.
+Definition SimEnv sitpn (γ : Sitpn2HVhdlMap sitpn) (E__c : nat -> C sitpn -> bool) (E__p : nat -> Clk -> IdMap value) : Prop :=
+  forall τ clk c id__c b,
+    (* [γ(c) = id__c] *)
+    SetoidList.InA Ckeq (c, id__c) (c2in γ)  ->
+    (* [E__p(τ,clk)(id__c) = E__c(τ)(c)] *)
+    MapsTo id__c (Vbool b) (E__p τ clk) -> 
+    E__c τ c = b.
 
-(** Defines the state similarity relation between an SITPN state and
-    a H-VHDL design state.
- *)
+(** Defines the general state similarity relation between an SITPN
+    state and a H-VHDL design state.  *)
 
-Definition SimState {sitpn} (γ : P sitpn + T sitpn -> ident) (s : SitpnState sitpn) (σ : DState) : Prop :=
+Definition SimState sitpn (γ : Sitpn2HVhdlMap sitpn) (s : SitpnState sitpn) (σ : DState) : Prop :=
 
-  (* Markings are similar. *)
-  
-  forall (p : P sitpn) id__p σ__p,
-    (* [id__p] is the identifier of the place component associated with
-       place [p] by the [γ] binder. *)
-    γ (inl p) = id__p ->
+  (* Markings are similar. *)  
+  (forall p id__p σ__p,
+      (* [id__p] is the identifier of the place component associated with
+         place [p] by the [γ] binder. *)
+      SetoidList.InA Pkeq (p, id__p) (p2pcomp γ) ->
 
-    (* [σ__p] is the current state of component [id__p] is the global design
-       state [σ]. *)
-    MapsTo id__p σ__p (compstore σ) ->
+      (* [σ__p] is the current state of component [id__p] is the global
+         design state [σ]. *)
+      MapsTo id__p σ__p (compstore σ) ->
 
-    (* Marking of place [p] at state [s] equals value of signal
-       [s_marking] at state [σ__p]. *)
-    MapsTo Place.s_marking (Vnat (M s p)) (sigstore σ__p).
+      (* Marking of place [p] at state [s] equals value of signal
+         [s_marking] at state [σ__p]. *)
+      MapsTo Place.s_marking (Vnat (M s p)) (sigstore σ__p))
 
-Notation "γ ⊢ s '∼' σ" := (SimState γ s σ) (at level 50).
+  (* Time counters are similar *)
+  /\ (forall (t : Ti sitpn) id__t σ__t n,
+         (* [id__t] is the identifier of the T component associated with
+            transition [t] by the [γ] binder. *)
+         SetoidList.InA Tkeq (proj1_sig t, id__t) (t2tcomp γ) ->
+         
+         (* [σ__t] is the current state of T component [id__t] is the global
+            design state [σ]. *)
+         MapsTo id__t σ__t (compstore σ) ->
+
+         (* Signal ["s_time_counter"] has value [(Vnat n)] at state [σ__t] *)
+         MapsTo Transition.s_time_counter (Vnat n) (sigstore σ__t) ->
+
+         (* Then, time counter similarity is: *)
+         (upper t = i+ /\ TcLeLower s t -> I s t = n) /\
+         (upper t = i+ /\ TcGtLower s t -> proj1_sig (lower t) = n) /\
+         (forall m, upper t = ninat m /\ TcGtUpper s t -> proj1_sig m = n) /\
+         (upper t <> i+ /\ TcLeUpper s t -> I s t = n))
+
+  (* Reset orders are similar. *)
+  /\ (forall (t : Ti sitpn) id__t σ__t,
+         (* [id__t] is the identifier of the T component associated with
+            transition [t] by the [γ] binder. *)
+         SetoidList.InA Tkeq (proj1_sig t, id__t) (t2tcomp γ) ->
+         
+         (* [σ__t] is the current state of T component [id__t] is the global
+            design state [σ]. *)
+         MapsTo id__t σ__t (compstore σ) ->
+
+         (* Signal ["s_reinit_time_counter"] equals [reset s t] at state [σ__t] *)
+         MapsTo Transition.s_reinit_time_counter (Vbool (reset s t)) (sigstore σ__t))
+
+  (* Action executions are similar. *)
+  /\ (forall a id__a,
+         (* [id__a] is the output port identifier associated to action
+            [a] in the [γ] binder. *)
+         SetoidList.InA Akeq (a, id__a) (a2out γ) ->
+         
+         (* Output port [id__a] equals [ex s (inl a)] at state [σ] *)
+         MapsTo id__a (Vbool (ex s (inl a))) (sigstore σ))
+
+  (* Function executions are similar. *)
+  /\ (forall f id__f,
+         (* [id__f] is the output port identifier associated to function
+            [f] in the [γ] binder. *)
+         SetoidList.InA Fkeq (f, id__f) (f2out γ) ->
+         
+         (* Output port [id__f] equals [ex s (inr f)] at state [σ] *)
+         MapsTo id__f (Vbool (ex s (inr f))) (sigstore σ))
+
+  (* Condition values are similar. *)
+  /\ (forall c id__c,
+         (* [id__c] is the input port identifier associated to condition
+            [c] in the [γ] binder. *)
+         SetoidList.InA Ckeq (c, id__c) (c2in γ) ->
+         
+         (* Input port [id__c] equals [cond s c] at state [σ] *)
+         MapsTo id__c (Vbool (cond s c)) (sigstore σ)).
+
+Notation "γ ⊢ s '∼' σ" := (SimState _ γ s σ) (at level 50).
+
+(** Defines the state similarity relation, after a rising edge,
+    between an SITPN state and a H-VHDL design state.  *)
+
+Definition SimStateAfterRE sitpn (γ : Sitpn2HVhdlMap sitpn) (s : SitpnState sitpn) (σ : DState) : Prop :=
+
+  (* Markings are similar. *)  
+  (forall p id__p σ__p,
+      (* [id__p] is the identifier of the place component associated with
+         place [p] by the [γ] binder. *)
+      SetoidList.InA Pkeq (p, id__p) (p2pcomp γ) ->
+
+      (* [σ__p] is the current state of component [id__p] is the global
+         design state [σ]. *)
+      MapsTo id__p σ__p (compstore σ) ->
+
+      (* Marking of place [p] at state [s] equals value of signal
+         [s_marking] at state [σ__p]. *)
+      MapsTo Place.s_marking (Vnat (M s p)) (sigstore σ__p))
+
+  (* Time counters are similar *)
+  /\ (forall (t : Ti sitpn) id__t σ__t n,
+         (* [id__t] is the identifier of the T component associated with
+            transition [t] by the [γ] binder. *)
+         SetoidList.InA Tkeq (proj1_sig t, id__t) (t2tcomp γ) ->
+         
+         (* [σ__t] is the current state of T component [id__t] is the global
+            design state [σ]. *)
+         MapsTo id__t σ__t (compstore σ) ->
+
+         (* Signal ["s_time_counter"] has value [(Vnat n)] at state [σ__t] *)
+         MapsTo Transition.s_time_counter (Vnat n) (sigstore σ__t) ->
+
+         (* Then, time counter similarity is: *)
+         (upper t = i+ /\ TcLeLower s t -> I s t = n) /\
+         (upper t = i+ /\ TcGtLower s t -> proj1_sig (lower t) = n) /\
+         (forall m, upper t = ninat m /\ TcGtUpper s t -> proj1_sig m = n) /\
+         (upper t <> i+ /\ TcLeUpper s t -> I s t = n))
+
+  (* Reset orders are similar. *)
+  /\ (forall (t : Ti sitpn) id__t σ__t,
+         (* [id__t] is the identifier of the T component associated with
+            transition [t] by the [γ] binder. *)
+         SetoidList.InA Tkeq (proj1_sig t, id__t) (t2tcomp γ) ->
+         
+         (* [σ__t] is the current state of T component [id__t] is the global
+            design state [σ]. *)
+         MapsTo id__t σ__t (compstore σ) ->
+
+         (* Signal ["s_reinit_time_counter"] equals [reset s t] at state [σ__t] *)
+         MapsTo Transition.s_reinit_time_counter (Vbool (reset s t)) (sigstore σ__t))
+
+  (* Action executions are similar. *)
+  /\ (forall a id__a,
+         (* [id__a] is the output port identifier associated to action
+            [a] in the [γ] binder. *)
+         SetoidList.InA Akeq (a, id__a) (a2out γ) ->
+         
+         (* Output port [id__a] equals [ex s (inl a)] at state [σ] *)
+         MapsTo id__a (Vbool (ex s (inl a))) (sigstore σ))
+
+  (* Function executions are similar. *)
+  /\ (forall f id__f,
+         (* [id__f] is the output port identifier associated to function
+            [f] in the [γ] binder. *)
+         SetoidList.InA Fkeq (f, id__f) (f2out γ) ->
+         
+         (* Output port [id__f] equals [ex s (inr f)] at state [σ] *)
+         MapsTo id__f (Vbool (ex s (inr f))) (sigstore σ))
+       
+  (* Sensitization is similar *)
+  /\ (forall t id__t σ__t,
+         (* [id__t] is the identifier of the T component associated with
+            transition [t] by the [γ] binder. *)
+         SetoidList.InA Tkeq (t, id__t) (t2tcomp γ) ->
+         
+         (* [σ__t] is the current state of T component [id__t] is the global
+            design state [σ]. *)
+         MapsTo id__t σ__t (compstore σ) ->
+
+         (* Signal ["s_enabled"] equals [true] is equivalent to t ∈ Sens(M). *)
+         Sens (M s) t <-> MapsTo Transition.s_enabled (Vbool true) (sigstore σ__t)).
+
+(** Defines the state similarity relation, after a falling edge,
+    between an SITPN state and a H-VHDL design state.  *)
+
+Definition SimStateAfterFE sitpn (γ : Sitpn2HVhdlMap sitpn) (s : SitpnState sitpn) (σ : DState) : Prop :=
+  γ ⊢ s ∼ σ 
+
+  (* Fired are similar. *)
+  /\ (forall t id__t σ__t fired,
+         (* [id__t] is the identifier of the T component associated with
+            transition [t] by the [γ] binder. *)
+         SetoidList.InA Tkeq (t, id__t) (t2tcomp γ) ->
+         
+         (* [σ__t] is the current state of T component [id__t] is the global
+            design state [σ]. *)
+         MapsTo id__t σ__t (compstore σ) ->
+
+         (* Output port ["fired"] equals [true] is equivalent to t ∈ Fired(s,fired). *)
+         Fired s fired t <-> MapsTo Transition.fired (Vbool true) (sigstore σ__t))
+       
+  (* Pre sum are similar. *)
+  /\ (forall p id__p σ__p fired pre__sum,
+         (* [id__p] is the identifier of the place component associated with
+            place [p] by the [γ] binder. *)
+         SetoidList.InA Pkeq (p, id__p) (p2pcomp γ) ->
+
+         (* [σ__p] is the current state of component [id__p] is the global
+            design state [σ]. *)
+         MapsTo id__p σ__p (compstore σ) ->
+
+         (* ∑ pre(p,t), for all t ∈ Fired(s). *)
+         PreSum p (Fired s fired) pre__sum -> 
+           
+         (* [∑ pre(p,t) = σ__p("s_output_token_sum")]. *)
+         MapsTo Place.s_output_token_sum (Vnat pre__sum) (sigstore σ__p))
+
+  (* Post sum are similar. *)
+  /\ (forall p id__p σ__p fired post__sum,
+         (* [id__p] is the identifier of the place component associated with
+            place [p] by the [γ] binder. *)
+         SetoidList.InA Pkeq (p, id__p) (p2pcomp γ) ->
+
+         (* [σ__p] is the current state of component [id__p] is the global
+            design state [σ]. *)
+         MapsTo id__p σ__p (compstore σ) ->
+
+         (* ∑ post(t,p), for all t ∈ Fired(s). *)
+         PostSum p (Fired s fired) post__sum -> 
+         
+         (* [∑ pre(p,t) = σ__p("s_output_token_sum")]. *)
+         MapsTo Place.s_output_token_sum (Vnat post__sum) (sigstore σ__p)).
 
 (** States that two execution trace are similar. The first list
     argument is the execution trace of an SITPN and the second list
@@ -89,67 +295,67 @@ Inductive SimTrace {sitpn} γ : list (SitpnState sitpn) -> list DState -> Prop :
         
  *)
 
-Inductive PastSimFalling (D : IdMap design) (M : IdMap value) (d : design) (Δ : ElDesign) : list DState -> DState -> Prop :=
-  PastSimFalling_cons :
-    forall σ__e θ σ σ__f,
-      (* Side conditions *)
-      edesign D M d Δ σ__e -> 
+(* Inductive PastSimFalling (D : IdMap design) (M : IdMap value) (d : design) (Δ : ElDesign) : list DState -> DState -> Prop := *)
+(*   PastSimFalling_cons : *)
+(*     forall σ__e θ σ σ__f, *)
+(*       (* Side conditions *) *)
+(*       edesign D M d Δ σ__e ->  *)
       
-      (* Premises *)
-      PastSimRisingStab D M d Δ θ σ ->
-      vfalling Δ σ (get_behavior d) σ__f ->
+(*       (* Premises *) *)
+(*       PastSimRisingStab D M d Δ θ σ -> *)
+(*       vfalling Δ σ (behavior d) σ__f -> *)
 
-      (* Conclusion *)
-      PastSimFalling D M d Δ (θ ++ [σ]) σ__f
+(*       (* Conclusion *) *)
+(*       PastSimFalling D M d Δ (θ ++ [σ]) σ__f *)
                      
-with PastSimRisingStab (D : IdMap design) (M : IdMap value) (d : design) (Δ : ElDesign) : list DState -> DState -> Prop :=
-| PastSimRisingStab_cons :
-    forall σ__e θ θ' σ σ',
-      (* Side conditions *)
-      edesign D M d Δ σ__e -> 
+(* with PastSimRisingStab (D : IdMap design) (M : IdMap value) (d : design) (Δ : ElDesign) : list DState -> DState -> Prop := *)
+(* | PastSimRisingStab_cons : *)
+(*     forall σ__e θ θ' σ σ', *)
+(*       (* Side conditions *) *)
+(*       edesign D M d Δ σ__e ->  *)
       
-      (* Premises *)
-      PastSimRising D M d Δ θ σ ->
-      stabilize Δ σ (get_behavior d) θ' σ' ->
+(*       (* Premises *) *)
+(*       PastSimRising D M d Δ θ σ -> *)
+(*       stabilize Δ σ (behavior d) θ' σ' -> *)
 
-      (* Conclusion *)
-      PastSimRisingStab D M d Δ (θ ++ [σ]) σ'
+(*       (* Conclusion *) *)
+(*       PastSimRisingStab D M d Δ (θ ++ [σ]) σ' *)
                         
-with PastSimRising (D : IdMap design) (M : IdMap value) (d : design) (Δ : ElDesign) : list DState -> DState -> Prop :=
-  PastSimRising_cons :
-    forall σ__e θ σ σ__r,
-      (* Side conditions *)
-      edesign D M d Δ σ__e -> 
+(* with PastSimRising (D : IdMap design) (M : IdMap value) (d : design) (Δ : ElDesign) : list DState -> DState -> Prop := *)
+(*   PastSimRising_cons : *)
+(*     forall σ__e θ σ σ__r, *)
+(*       (* Side conditions *) *)
+(*       edesign D M d Δ σ__e ->  *)
       
-      (* Premises *)
-      PastSimFallingStab D M d Δ θ σ ->
-      vrising Δ σ (get_behavior d) σ__r ->
+(*       (* Premises *) *)
+(*       PastSimFallingStab D M d Δ θ σ -> *)
+(*       vrising Δ σ (behavior d) σ__r -> *)
 
-      (* Conclusion *)
-      PastSimRising D M d Δ (θ ++ [σ]) σ__r
+(*       (* Conclusion *) *)
+(*       PastSimRising D M d Δ (θ ++ [σ]) σ__r *)
                      
-with PastSimFallingStab (D : IdMap design) (M : IdMap value) (d : design) (Δ : ElDesign)  : list DState -> DState -> Prop :=
-| PastSimFallingStab_init :
-    forall σ__e σ0,
-      (* Side conditions *)
-      edesign D M d Δ σ__e -> 
+(* with PastSimFallingStab (D : IdMap design) (M : IdMap value) (d : design) (Δ : ElDesign)  : list DState -> DState -> Prop := *)
+(* | PastSimFallingStab_init : *)
+(*     forall σ__e σ0, *)
+(*       (* Side conditions *) *)
+(*       edesign D M d Δ σ__e ->  *)
 
-      (* Premises *)
-      init Δ σ__e (get_behavior d) σ0 ->
+(*       (* Premises *) *)
+(*       init Δ σ__e (behavior d) σ0 -> *)
 
-      (* Conclusion *)
-      PastSimFallingStab D M d Δ [] σ0
+(*       (* Conclusion *) *)
+(*       PastSimFallingStab D M d Δ [] σ0 *)
                          
-| PastSimFallingStab_cons :
-    forall σ__e θ θ' σ σ',
-      (* Side conditions *)
-      edesign D M d Δ σ__e -> 
+(* | PastSimFallingStab_cons : *)
+(*     forall σ__e θ θ' σ σ', *)
+(*       (* Side conditions *) *)
+(*       edesign D M d Δ σ__e ->  *)
       
-      (* Premises *)
-      PastSimFalling D M d Δ θ σ ->
-      stabilize Δ σ (get_behavior d) θ' σ' ->
+(*       (* Premises *) *)
+(*       PastSimFalling D M d Δ θ σ -> *)
+(*       stabilize Δ σ (behavior d) θ' σ' -> *)
 
-      (* Conclusion *)
-      PastSimFallingStab D M d Δ (θ ++ [σ]) σ'.
+(*       (* Conclusion *) *)
+(*       PastSimFallingStab D M d Δ (θ ++ [σ]) σ'. *)
 
 
