common/InAndNoDup.v
@@ -10,7 +10,9 @@ Require Import FstSplit.
 Section InAndNoDupLemmas.
 
   (* In tail of list *)
-  Lemma in_last {A : Type} : forall (a : A) l, In a (l ++ [a]). firstorder. Defined.
+  Lemma in_last {A : Type} : forall (a : A) l, In a (l ++ [a]).
+    intros; apply in_elt.
+  Defined.
   
   (** If a is in list l and l is in list of lists ll then a is in (concat ll).
       The result of (concat ll) is one list corresponding
