soundness/Soundness.v
@@ -2,14 +2,15 @@
 
 Require Import NatMap.
 
-Require Import Coqlib.
-Require Import InAndNoDup.
-Require Import GlobalTypes.
-Require Import ListsPlus.
-Require Import SitpnSemanticsDefs.
+Require Import common.Coqlib.
+Require Import common.InAndNoDup.
+Require Import common.GlobalTypes.
+Require Import common.ListsPlus.
+
 
 (* SITPN Libraries *)
 
+Require Import dp.SitpnSemanticsDefs.
 Require Import dp.SitpnTypes.
 Require Import dp.Sitpn.
 Require Import dp.SitpnSemantics.
@@ -17,28 +18,26 @@ Require Import dp.Fired.
 
 (* H-VHDL Libraries *)
 
-Require Import HVhdlTypes.
-Require Import Environment.
-Require Import SemanticalDomains.
-Require Import Simulation.
-Require Import CombinationalEvaluation.
-Require Import SynchronousEvaluation.
-Require Import DesignElaboration.
-Require Import AbstractSyntax.
-Require Import HilecopDesignStore.
-Require Import Initialization.
-Require Import Stabilize.
-Require Import PortMapEvaluation.
+Require Import hvhdl.HVhdlTypes.
+Require Import hvhdl.Environment.
+Require Import hvhdl.SemanticalDomains.
+Require Import hvhdl.Simulation.
+Require Import hvhdl.CombinationalEvaluation.
+Require Import hvhdl.SynchronousEvaluation.
+Require Import hvhdl.DesignElaboration.
+Require Import hvhdl.AbstractSyntax.
+Require Import hvhdl.HilecopDesignStore.
+Require Import hvhdl.Initialization.
+Require Import hvhdl.Stabilize.
+Require Import hvhdl.PortMapEvaluation.
 
 (* SITPN to H-VHDL Libraries *)
 
-Require Import GenerateHVhdl.
+Require Import sitpn2hvhdl.GenerateHVhdl.
 
 (* Soundness definitions and lemmas *)
 
-Require Import SoundnessDefs.
-Require Import RisingEdgeFacts.
-Require Import FallingEdgeFacts.
+Require Import soundness.SoundnessDefs.
 
 Local Unset Implicit Arguments.
 
@@ -49,193 +48,193 @@ Local Unset Implicit Arguments.
 
  *)
 
-Lemma step_lemma :
-  forall sitpn decpr mm d s s' E__c σ σ' Δ Mg σ__e P__i τ γ,
+(* Lemma step_lemma : *)
+(*   forall sitpn decpr id__ent id__arch mm d s s' E__c σ σ' Δ Mg σ__e P__i τ γ, *)
     
-    (* sitpn translates into d. *)
-    sitpn_to_hvhdl sitpn decpr mm = Success d ->
+(*     (* sitpn translates into d. *) *)
+(*     sitpn_to_hvhdl sitpn decpr id__ent id__arch mm = (inl (d, γ)) -> *)
 
-    (* Starting states are similar *)
-    γ ⊢ s ∼ σ ->
+(*     (* Starting states are similar *) *)
+(*     γ ⊢ s ∼ σ -> *)
 
-    (* [Δ, σ__e] are the results of the elaboration of [d]. *)
-    edesign hdstore Mg d Δ σ__e ->
+(*     (* [Δ, σ__e] are the results of the elaboration of [d]. *) *)
+(*     edesign hdstore Mg d Δ σ__e -> *)
     
-    (* One execution cycle for SITPN *)
+(*     (* One execution cycle for SITPN *) *)
     
-    @SitpnCycle sitpn E__c τ s s' ->
+(*     @SitpnCycle sitpn E__c τ s s' -> *)
 
-    (* One execution cycle for VHDL *)
-    simcycle P__i Δ τ σ (get_behavior d) σ' ->
+(*     (* One execution cycle for VHDL *) *)
+(*     simcycle P__i Δ τ σ (behavior d) σ' -> *)
      
-    (* Final states are similar *)
-    γ ⊢ s' ∼ σ'.
-Proof.
-  intros *; intros Htransl Hsim Helab Hsitpn_cyc Hhdl_cyc.
-  unfold SitpnCycle in Hsitpn_cyc.
-  inversion_clear Hsitpn_cyc as (s__i & (Hrising, Hfalling)).
-  inversion_clear Hhdl_cyc as
-      (σ__injr, σ__r, σ__i, σ__injf, σ__f, σ'', θ, θ',
-       Hhdl_rising, Hstab_rising, Hhdl_falling, Hstab_falling, Hinj_rising, Hinj_falling).
+(*     (* Final states are similar *) *)
+(*     γ ⊢ s' ∼ σ'. *)
+(* Proof. *)
+(*   intros *; intros Htransl Hsim Helab Hsitpn_cyc Hhdl_cyc. *)
+(*   unfold SitpnCycle in Hsitpn_cyc. *)
+(*   inversion_clear Hsitpn_cyc as (s__i & (Hrising, Hfalling)). *)
+(*   inversion_clear Hhdl_cyc as *)
+(*       (σ__injr, σ__r, σ__i, σ__injf, σ__f, σ'', θ, θ', *)
+(*        Hhdl_rising, Hstab_rising, Hhdl_falling, Hstab_falling, Hinj_rising, Hinj_falling). *)
 
-  (* Must prove s similar to σ after capture of input values on rising edge. 
-     Necessary premise to apply [rising_edge_states_equal].      
-   *)
-  cut (γ ⊢ s ∼ σ__injr); intros Hsim_injr.
-  specialize (rising_edge_states_equal
-           Δ σ__r d θ σ__i σ__injr sitpn decpr E__c τ s s__i mm γ
-           Htransl Hsim_injr Hrising Hhdl_rising Hstab_rising); intros Heq_int_states.
+(*   (* Must prove s similar to σ after capture of input values on rising edge.  *)
+(*      Necessary premise to apply [rising_edge_states_equal].       *)
+(*    *) *)
+(*   cut (γ ⊢ s ∼ σ__injr); intros Hsim_injr. *)
+(*   specialize (rising_edge_states_equal *)
+(*            Δ σ__r d θ σ__i σ__injr sitpn decpr E__c τ s s__i mm γ *)
+(*            Htransl Hsim_injr Hrising Hhdl_rising Hstab_rising); intros Heq_int_states. *)
 
-  (* Must prove s similar to σ after capture of input values on falling edge. 
-     Necessary premise to apply [falling_edge_states_equal].
-   *)
-  cut (γ ⊢ s__i ∼ σ__injf); intros Hsim_injf.
-  apply (falling_edge_states_equal Δ σ__f d θ' σ' σ__injf sitpn decpr E__c τ s__i s' mm γ
-                                   Htransl Hsim_injf Hfalling Hhdl_falling Hstab_falling).
+(*   (* Must prove s similar to σ after capture of input values on falling edge.  *)
+(*      Necessary premise to apply [falling_edge_states_equal]. *)
+(*    *) *)
+(*   cut (γ ⊢ s__i ∼ σ__injf); intros Hsim_injf. *)
+(*   apply (falling_edge_states_equal Δ σ__f d θ' σ' σ__injf sitpn decpr E__c τ s__i s' mm γ *)
+(*                                    Htransl Hsim_injf Hfalling Hhdl_falling Hstab_falling). *)
   
-  - admit.
-  - admit.
-Admitted.
+(*   - admit. *)
+(*   - admit. *)
+(* Admitted. *)
 
 (** ** Equal Initial States  *)
 
-Lemma init_states_sim :
-  forall sitpn decpr mm d Δ σ__e σ0 γ,
+(* Lemma init_states_sim : *)
+(*   forall sitpn decpr mm d Δ σ__e σ0 γ, *)
     
-    (* sitpn translates into d. *)
-    sitpn_to_hvhdl sitpn decpr mm = Success d ->
+(*     (* sitpn translates into d. *) *)
+(*     sitpn_to_hvhdl sitpn decpr mm = Success d -> *)
 
-    (* ed, dstate are the results of the elaboration of d. *)
-    edesign hdstore (empty value) d Δ σ__e ->
+(*     (* ed, dstate are the results of the elaboration of d. *) *)
+(*     edesign hdstore (empty value) d Δ σ__e -> *)
 
-    (* initialization d's state. *)
-    init Δ σ__e (get_behavior d) σ0 ->
+(*     (* initialization d's state. *) *)
+(*     init Δ σ__e (get_behavior d) σ0 -> *)
 
-    (* init states are similar *)
-    γ ⊢ (s0 sitpn) ∼ σ0.
-Proof.
-  intros *; intros Htransl Helab Hinit.
-  inversion_clear Hinit as (σ, beh, σ', σ'', θ, Hruninit, Hstab).
+(*     (* init states are similar *) *)
+(*     γ ⊢ (s0 sitpn) ∼ σ0. *)
+(* Proof. *)
+(*   intros *; intros Htransl Helab Hinit. *)
+(*   inversion_clear Hinit as (σ, beh, σ', σ'', θ, Hruninit, Hstab). *)
 
-Admitted.
+(* Admitted. *)
 
 (** ** Similar States after First Cycle  *)
 
-Lemma sim_after_first_cycle :
-  forall sitpn decpr mm d E__c E__p Δ σ__e σ0 τ σ s γ,
-    (* [sitpn] translates into [d]. *)
-    sitpn_to_hvhdl sitpn decpr mm = Success d ->
+(* Lemma sim_after_first_cycle : *)
+(*   forall sitpn decpr mm d E__c E__p Δ σ__e σ0 τ σ s γ, *)
+(*     (* [sitpn] translates into [d]. *) *)
+(*     sitpn_to_hvhdl sitpn decpr mm = Success d -> *)
 
-    (* Environments are similar. *)
-    EnvEq sitpn E__c E__p ->
+(*     (* Environments are similar. *) *)
+(*     EnvEq sitpn E__c E__p -> *)
 
-    (* [Δ, σ__e] are the results of the elaboration of [d]. *)
-    edesign hdstore (empty value) d Δ σ__e ->
+(*     (* [Δ, σ__e] are the results of the elaboration of [d]. *) *)
+(*     edesign hdstore (empty value) d Δ σ__e -> *)
 
-    (* [σ0] is the initial state of [d]. *)
-    init Δ σ__e (get_behavior d) σ0 ->
+(*     (* [σ0] is the initial state of [d]. *) *)
+(*     init Δ σ__e (get_behavior d) σ0 -> *)
 
-    (* From [σ0] to [σ] in one simulation cycle. *)
-    simcycle E__p Δ (S τ) σ0 (get_behavior d) σ ->
+(*     (* From [σ0] to [σ] in one simulation cycle. *) *)
+(*     simcycle E__p Δ (S τ) σ0 (get_behavior d) σ -> *)
 
-    (* From [s0] to [s] in one execution cycle, where [Fired(s0) = ∅]. *)
-    SitpnStateTransition E__c (S τ) (s0 sitpn) s falling_edge ->
+(*     (* From [s0] to [s] in one execution cycle, where [Fired(s0) = ∅]. *) *)
+(*     SitpnStateTransition E__c (S τ) (s0 sitpn) s falling_edge -> *)
 
-    (* States [s] and [σ] are similar. *)
-    γ ⊢ s ∼ σ.
-Admitted.
+(*     (* States [s] and [σ] are similar. *) *)
+(*     γ ⊢ s ∼ σ. *)
+(* Admitted. *)
 
 (** ** Simulation Lemma *)
 
-Lemma simulation_lemma :
+(* Lemma simulation_lemma : *)
   
-  forall sitpn Ec τ s θ__s s',
+(*   forall sitpn Ec τ s θ__s s', *)
 
-    (* From state s to state s' after τ execution cycles, and
-       producing trace θs. *)
-    SitpnExecute Ec s τ θ__s s' ->
+(*     (* From state s to state s' after τ execution cycles, and *)
+(*        producing trace θs. *) *)
+(*     SitpnExecute Ec s τ θ__s s' -> *)
 
-    forall decpr d mm Ep Δ σ__e θ__σ σ σ' γ,
+(*     forall decpr d mm Ep Δ σ__e θ__σ σ σ' γ, *)
       
-    (* sitpn translates into d. *)
-    sitpn_to_hvhdl sitpn decpr mm = Success d ->
+(*     (* sitpn translates into d. *) *)
+(*     sitpn_to_hvhdl sitpn decpr mm = Success d -> *)
 
-    (* Environments are similar. *)
-    EnvEq sitpn Ec Ep ->
+(*     (* Environments are similar. *) *)
+(*     EnvEq sitpn Ec Ep -> *)
 
-    (* Δ, σe are the results of the elaboration of d. *)
-    edesign hdstore (empty value) d Δ σ__e ->
+(*     (* Δ, σe are the results of the elaboration of d. *) *)
+(*     edesign hdstore (empty value) d Δ σ__e -> *)
 
-    (* States s and σ are similar; *)
-    γ ⊢ s ∼ σ ->
+(*     (* States s and σ are similar; *) *)
+(*     γ ⊢ s ∼ σ -> *)
     
-    (* From [σ] to [σ'] after τ execution cycles, producing trace [θ__σ]. *)
-    simloop Ep Δ σ (get_behavior d) τ θ__σ σ' ->
+(*     (* From [σ] to [σ'] after τ execution cycles, producing trace [θ__σ]. *) *)
+(*     simloop Ep Δ σ (get_behavior d) τ θ__σ σ' -> *)
 
-    (* Conclusion *)
-    SimTrace γ θ__s θ__σ.
-Proof.
-  intros *; intros Hexec; dependent induction Hexec;
-  intros *; intros Htransl Henveq Helab Hsimstate Hsim.
+(*     (* Conclusion *) *)
+(*     SimTrace γ θ__s θ__σ. *)
+(* Proof. *)
+(*   intros *; intros Hexec; dependent induction Hexec; *)
+(*   intros *; intros Htransl Henveq Helab Hsimstate Hsim. *)
   
-  (* CASE tau = 0, trivial. *)
-  - inversion Hsim; apply SimTraceInit.
+(*   (* CASE tau = 0, trivial. *) *)
+(*   - inversion Hsim; apply SimTraceInit. *)
 
-  (* CASE tau > 0 *)
-  - inversion_clear Hsim as [ τ0 σ0 σ'0 θ0 Hcyc Hsiml |  ].
+(*   (* CASE tau > 0 *) *)
+(*   - inversion_clear Hsim as [ τ0 σ0 σ'0 θ0 Hcyc Hsiml |  ]. *)
     
-    (* Specializes the induction hypothesis, then apply the step lemma. *)
+(*     (* Specializes the induction hypothesis, then apply the step lemma. *) *)
     
-    specialize (IHHexec decpr d mm Ep Δ σ__e θ0 σ0 σ').
-    specialize (IHHexec γ Htransl Henveq Helab).
+(*     specialize (IHHexec decpr d mm Ep Δ σ__e θ0 σ0 σ'). *)
+(*     specialize (IHHexec γ Htransl Henveq Helab). *)
 
-    (* Then, we need a lemma stating that s' ∼ σ0. That is, state are
-       similar after one execution cycle. *)
+(*     (* Then, we need a lemma stating that s' ∼ σ0. That is, state are *)
+(*        similar after one execution cycle. *) *)
 
-    specialize (step_lemma sitpn decpr mm d s s' Ec σ σ0 Δ (empty value) σ__e Ep (S τ) γ
-                           Htransl Hsimstate Helab H Hcyc)
-      as Heq_state_cyc.
+(*     specialize (step_lemma sitpn decpr mm d s s' Ec σ σ0 Δ (empty value) σ__e Ep (S τ) γ *)
+(*                            Htransl Hsimstate Helab H Hcyc) *)
+(*       as Heq_state_cyc. *)
 
-    (* Solve the induction case. *)
-    apply (@SimTraceCons sitpn γ s' σ0 θ θ0);
-      [ assumption | apply (IHHexec Heq_state_cyc Hsiml)].
-Qed.
+(*     (* Solve the induction case. *) *)
+(*     apply (@SimTraceCons sitpn γ s' σ0 θ θ0); *)
+(*       [ assumption | apply (IHHexec Heq_state_cyc Hsiml)]. *)
+(* Qed. *)
 
 (** ** Semantic Preservation Theorem *)
 
 Theorem sitpn2vhdl_sound :
-  forall sitpn decpr E__c τ θ__s d E__p mm θ__σ γ,
+  forall sitpn decpr id__ent id__arch E__c τ θ__s d E__p mm θ__σ γ Δ,
       
     (* sitpn translates into d. *)
-    sitpn_to_hvhdl sitpn decpr mm = Success d ->
+    sitpn_to_hvhdl sitpn decpr id__ent id__arch mm = (inl (d, γ)) ->
 
     (* Environments are similar. *)
-    EnvEq sitpn E__c E__p ->
+    SimEnv sitpn γ E__c E__p ->
     
     (* SITPN [sitpn] yields execution trace [θ__s] after [τ] execution cycles. *)
     
-    @SitpnExecWf sitpn E__c τ θ__s ->    
+    @SitpnFullExec sitpn E__c τ θ__s ->    
 
     (* Design [d] yields simulation trace [θ__σ] after [τ] simulation cycles. *)
-    hsimwf d E__p τ θ__σ ->
+    hfullsim E__p τ Δ d θ__σ ->
     
     (* ** Conclusion: traces are positionally similar. ** *)
     SimTrace γ θ__s θ__σ.
 Proof.
   intros.
-
+  
   lazymatch goal with
   | [
-    Htransl: sitpn_to_hvhdl _ _ _ = _,
-    Henveq: EnvEq _ _ _,
-    Hsitpnexecwf: @SitpnExecWf _ _ _ _,
-    Hsimwf: hsimwf _ _ _ _
+    Htransl: sitpn_to_hvhdl _ _ _ _ _ = _,
+    Hsenv: @SimEnv _ _ _ _,
+    Hsitpnfexec: @SitpnFullExec _ _ _ _,
+    Hhfsim: hfullsim _ _ _ _ _
     |- _ ] =>
     
     (* CASE τ = 0, traces are empty. Trivial. *)
-    destruct τ; inversion_clear Hsitpnexecwf; inversion_clear Hsimwf; [
-      apply SimTraceInit |
-      auto
+    destruct τ; inversion_clear Hsitpnfexec; inversion_clear Hhfsim; [
+      eauto |
+      eauto
     ]
   end.
 
